# Proof 0A = 0

We have A0 = 0 and 0 + A = A + 0 = 0, so all that remains is 0A = 0

Also, `0a = 0` was proven for reals as follows:

If 0a is not 0, it has an inverse (non-zero reals have an inverse), so we get:

1. (0a)x = 1
2. 2(0a)x = 2
3. 2(0a)x = (0a)x (because 2(0) = 0)

A contradiction!

Unfortunately, non-zero _complex_ numbers do not necessarily have an inverse at the moment.

However, we do have `_i _i _i _i = 1`, so numbers of the form `_i r` have an inverse.

We know `0A = a + _i b`, and `0A has inverse -> 0A = 0`

If either `a` or `b` is `0`, `0A` would have an inverse, so `a` and `b` are non-zero and have inverse.

Finally, `0A = 0` if `0i = 0` since `0A = 0r + 0is`

Now...

```
            0i  = a + ib
   -a   +   0i  =     ib
 i(-a)  + i(0i) =    iib
 i(-a)  +   0i  =  (-1)b
0i(-a)  +   0i  = 0(-1)b
0i(-a)  +   0i   = 0
0(i(-a) +    i)   = 0
0(i(-a) +    i(1)) = 0
0(i(-a  +    1))   = 0

If (-a + 1) has an inverse:
  0i(-a + 1)((-a + 1)^-1) = 0i = 0

So (-a + 1) is 0, and a = 1
```

```
0i = 1 + ib
0i + i(-b) = 1
00i + 0i(-b) = 01
0i + 0i(-b) = 0
0(i(1 + -b)) = 0

Similarly b = 1
```

```
0i = 1 + i1
   = 1 + i

iii0i = iii(1 + i)
      = iii + iiii
      = -i + 1
iii0i = 0i
   0i = -i + 1

0i + 0i = (1 + i) + (-i + 1)
        = 1 + 1
0i(1 + 1) = 1(1 + 1)
0i(1 + 1)((1 + 1)^-1) = 1(1 + 1)((1 + 1)^-1)
0i = 1
00i = 0i = 01 = 0
0i = 0
```
